\begin{frame}
  \begin{itemize}[<+->]
    \item purely functional data structure
    \item \mintinline{Haskell}{(<|)} and \mintinline{Haskell}{viewL} in \(\Theta(1)\)
    \item concatenation in \(\Theta(\log(\min\{n_1,n_2\}))\)
    \item splitting in \(\Theta(\log(\min\{n_l,n_r\}))\)
    \item general purpose
  \end{itemize}
\end{frame}


\begin{frame}[fragile]
\begin{minted}{Haskell}
data Digit a =
    One a 
  | Two a a 
  | Three a a a 
  | Four a a a a
data FingerTree v a =
    Empty
  | Single a
  | Deep v (Digit a) (FingerTree v (Node v a)) (Digit a)

(><) :: Measured a v => FingerTree v a -> FingerTree v a
  -> FingerTree v a
split :: Measured a v => (v -> Bool) -> FingerTree v a 
  -> (FingerTree v a, FingerTree v a)
  \end{minted}
\end{frame}

\subsection{Elementary Operations}
\begin{frame}[fragile]
  \begin{minted}{Haskell}
(.+|) :: Measured a v => v -> a -> v
i .+| s = i <> μ s

node3 :: Measured a v => a -> a -> a -> Node v a
node3 a b c = Node3 (μ a .+| b .+| c) a b c

instance Measured a v =>
  Extendable a (FingerTree v) where
    a <| Empty = Single a
    a <| Single b = deep (One a) Empty (One b)
    a <| Deep _ (Four b c d e) m sf =
        deep (Two a b) (node3 c d e <| m) sf
    a <| Deep _ pr m sf = deep (a <| pr) m sf
  \end{minted}
\end{frame}

\begin{frame}
  Big Example
\end{frame}

\begin{frame}[fragile]
  \begin{minted}{Haskell}
instance Measured a v => 
  Viewable a (FingerTree v) where
    viewL Empty = Nil
    viewL (Single x) = Cons x Empty
    viewL (Deep _ pr m sf) = case viewL pr of
        Nil -> let 
            One a = pr 
          in Cons a (case viewL m of
            Nil -> toTree sf
            Cons b m -> deep (nodeTodigit b) m sf)
        Cons a pr -> Cons a (deep pr m sf)
  \end{minted}
\end{frame}

\subsection{Concatenate}
\begin{frame}[fragile]
  \begin{minted}{Haskell}
nodes :: Measured a v => [a] -> [Node v a]
nodes [a,b] = [node2 a b]
nodes [a,b,c] = [node3 a b c]
nodes [a,b,c,d] = [node2 a b, node2 c d]
nodes (a:b:c:xs) = node3 a b c : nodes xs

app3 :: Measured a v => FingerTree v a -> [a]
  -> FingerTree v a -> FingerTree v a
app3 Empty ts xs = ts <|| xs
app3 xs ts Empty = xs ||> ts
app3 (Single x) ts xs = x <| (ts <|| xs)
app3 xs ts (Single x) = (xs ||> ts) |> x
app3 (Deep _ pr1 m1 sf1) ts (Deep _ pr2 m2 sf2) =
  deep
    pr1 
    (app3 m1 (nodes (sf1 <|| (ts ||> pr2))) m2)
    sf2
  \end{minted}
\end{frame}

\begin{frame}[fragile]
  \begin{minted}{Haskell}
(><) :: Measured a v => FingerTree v a -> FingerTree v a
  -> FingerTree v a
xs >< ys = app3 xs [] ys
  \end{minted}
\end{frame}

\subsection{Split}
\begin{frame}[fragile]
\begin{minted}{Haskell}
data Split f a = Split (f a) a (f a)

deepL :: Measured a v => [a] -> FingerTree v (Node v a)
    -> Digit a -> FingerTree v a
deepL [] m sf = case viewL m of
        Nil -> toTree sf
        Cons a m -> deep (nodeTodigit a) m sf
deepL (p:pr) m sf = deep (One p ||> pr) m sf
\end{minted}
\end{frame}

\begin{frame}[fragile]
\begin{minted}{Haskell}
splitTree :: Measured a v => (v -> Bool) -> v ->
    FingerTree v a -> Split (FingerTree v) a
splitTree _ _ (Single x) = Split Empty x Empty
splitTree p i (Deep _ pr m sf)
    | p vpr = let Split l x r = splitDigit p i pr 
        in Split (toTree l) x (deepL r m sf)
    | p vm = let
            Split ml xs mr = splitTree p vpr m
            Split l x r = splitDigit p (vpr .+| ml)
                (nodeTodigit xs)
        in
            Split (deepR pr ml l) x (deepL r mr sf)
    | otherwise = let Split l x r = splitDigit p vm sf
        in Split (deepR pr m l) x (toTree r)
    where
        vpr = i .+| pr
        vm = vpr .+| m
\end{minted}
\end{frame}

\begin{frame}[fragile]
\begin{minted}{Haskell}
split :: Measured a v => (v -> Bool) -> FingerTree v a
    -> (FingerTree v a, FingerTree v a)
split _ Empty = (Empty, Empty)
split p xs
    | p (μ xs) = let Split l x r = splitTree p mempty xs
        in (l, x <| r)
    | otherwise = (xs, Empty)
\end{minted}
\end{frame}

\begin{frame}[fragile]
\begin{minted}{Haskell}
lookupTree :: Measured a v => (v -> Bool) -> v ->
    FingerTree v a -> (v, a)
lookupTree _ i (Single x) = (i, x)
lookupTree p i (Deep _ pr m sf)
    | p vpr = lookupDigit p i pr
    | p vm = let (i', t) = lookupTree p vpr m
        in lookupNode p i' t
    | otherwise = lookupDigit p vm sf
    where
        vpr = i .+| pr
        vm = vpr .+| m
\end{minted}
\end{frame}